Finished arch sem soundness proof

hol/p4Lib.sig
@@ -11,5 +11,6 @@ val find_clause : thm -> string -> thm option
 val find_clause_e_red : string -> thm option
 val find_clause_stmt_red : string -> thm option
 val find_clause_frames_red : string -> thm option
+val find_clause_arch_red : string -> thm option
 
 end
