hol/p4Lib.sml
@@ -109,5 +109,7 @@ val find_clause_e_red = find_clause e_red_rules
 val find_clause_stmt_red = find_clause stmt_red_rules
 (* find_clause, hard-coded for the frame reduction theorem *)
 val find_clause_frames_red = find_clause frames_red_rules
+(* find_clause, hard-coded for the architecture-level reduction theorem *)
+val find_clause_arch_red = find_clause arch_red_rules
 
 end
